Byzantine network semantics

LeanSts/BFT/Network.lean
@@ -1,15 +1,22 @@
 import Mathlib.Tactic
 import LeanSts.BFT.Byzantine
 
-class NetworkPacket {NetAddr Message Packet : Type} :=
-  src : Packet → NetAddr
-  dst : Packet → NetAddr
-  msg : Packet → Message
+structure NetworkPacket {NetAddr Message : Type} :=
+  src : NetAddr
+  dst : NetAddr
+  msg : Message
+  consumed: Bool
+deriving DecidableEq
 
-class NetworkProtocol {NetAddr Message Packet LocalState InternalTransition : Type} :=
+abbrev Packet (NetAddr Message : Type) := @NetworkPacket NetAddr Message
+
+def receive (p : Packet NetAddr Message) : Packet NetAddr Message :=
+  { p with consumed := true }
+
+class NetworkProtocol {NetAddr Message LocalState InternalTransition : Type} :=
   localInit : NetAddr → LocalState
-  procInternal : LocalState → InternalTransition → LocalState × List Packet
-  procMessage : LocalState → NetAddr /- sender -/ → Message → LocalState × List Packet
+  procInternal : LocalState → InternalTransition → LocalState × List (Packet NetAddr Message)
+  procMessage : LocalState → NetAddr /- sender -/ → Message → LocalState × List (Packet NetAddr Message)
 
 /-- A network consists of the packet soup and the local states of nodes.
   Informally, this is called a "World". -/
@@ -19,16 +26,19 @@ structure NetworkState {NetAddr Packet LocalState : Type} :=
   /-- The set of sent messages. -/
   packetSoup : Multiset Packet
 
+def consume [DecidableEq (Packet NetAddr Message)] (p : Packet NetAddr Message) (soup : Multiset (Packet NetAddr Message)) : Multiset (Packet NetAddr Message) :=
+  (soup.erase p) + {receive p}
+
+@[simp] def updNS {NetAddr LocalState : Type} [DecidableEq NetAddr]
+  (n : NetAddr) (st : LocalState) (states : NetAddr → LocalState) : NetAddr → LocalState :=
+  λ n' => if n = n' then st else states n'
+
 theorem defaultNetworkState
-  [protocol : @NetworkProtocol NetAddr Message Packet LocalState InternalTransition]
-  : Inhabited (@NetworkState NetAddr Packet LocalState) :=
+  [protocol : @NetworkProtocol NetAddr Message LocalState InternalTransition]
+  : Inhabited (@NetworkState NetAddr (Packet NetAddr Message) LocalState) :=
   ⟨{ localState := λ n => protocol.localInit n, packetSoup := ∅ }⟩
 
-structure AsynchronousNetwork {NetAddr Message Packet LocalState InternalTransition : Type}
-  [pkt : @NetworkPacket NetAddr Message Packet]
-  [protocol : @NetworkProtocol NetAddr Message Packet LocalState InternalTransition]
-  [byz : @ByzantineAdversary NetAddr Message (@NetworkState NetAddr Packet LocalState)] :=
-
+namespace AsynchronousNetwork
   abbrev World {NetAddr Packet LocalState : Type} := @NetworkState NetAddr Packet LocalState
 
   /-- Description of a step being taken. -/
@@ -44,15 +54,37 @@ structure AsynchronousNetwork {NetAddr Message Packet LocalState InternalTransit
 
   /-- Transition relation of this network. -/
   inductive transition
-    [pkt : @NetworkPacket NetAddr Message Packet]
-    [protocol : @NetworkProtocol NetAddr Message Packet LocalState InternalTransition]
-    [byz : @ByzantineAdversary NetAddr Message (@NetworkState NetAddr Packet LocalState)]
-    (s : @step NetAddr Message Packet InternalTransition) (w w' : @World NetAddr Packet LocalState)
+    [DecidableEq NetAddr] [DecidableEq Message]
+    [protocol : @NetworkProtocol NetAddr Message LocalState InternalTransition]
+    [byz : @ByzantineAdversary NetAddr Message (@NetworkState NetAddr (Packet NetAddr Message) LocalState)]
+    (s : @step NetAddr Message (Packet NetAddr Message) InternalTransition)
+    (w w' : @World NetAddr (Packet NetAddr Message) LocalState)
+    /-- Stuttering. -/
     | idle (_ : s = step.idle) (_ : w = w')
-    | deliver (p : Packet)
+
+    /-- Packet `p` is delivered to its recipient. -/
+    | deliver (p : (Packet NetAddr Message))
       (_ : s = step.deliver p)
       (_ : p ∈ w.packetSoup)
-      (_ : ¬ byz.setting.isByzantine (pkt.dst p) w)
+      (_ : ¬ byz.setting.isByzantine p.dst w)
+      (_ : let (st', msgs) := protocol.procMessage (w.localState p.dst) p.src p.msg
+          w' = { w with localState := updNS p.dst st' w.localState,
+                        packetSoup := consume p w.packetSoup + msgs })
 
+    /-- Node `proc` executes internal transition `t`. -/
+    | intern (proc : NetAddr) (t : InternalTransition)
+      (_ : s = step.intern proc t)
+      (_ : ¬ byz.setting.isByzantine proc w)
+      (_ : let (st', msgs) := protocol.procInternal (w.localState proc) t
+          w' = { w with localState := updNS proc st' w.localState,
+                        packetSoup := w.packetSoup + msgs })
 
-#check AsynchronousNetwork
+    /-- The Byzantine adversary creates a message. -/
+    | byzantine (src dst : NetAddr) (msg : Message)
+      (_ : s = step.byz src dst msg)
+      (_ : byz.setting.isByzantine src w)
+      (_ : byz.constraint.canProduceMessage msg w)
+      (_ : let pkt := { src := src, dst := dst, msg := msg, consumed := false }
+        w' = { w with packetSoup := w.packetSoup + {pkt}})
+
+end AsynchronousNetwork
